[NSL]: Simplify specification.

examples/nsl.v
@@ -19,7 +19,7 @@ Section NSL.
 Context `{!heapGS Σ, !cryptisGS Σ, !tlockG Σ}.
 Notation iProp := (iProp Σ).
 
-Implicit Types (rl : role) (t kI kR nI nR sI sR kS : term).
+Implicit Types (rl : role) (t skI skR nI nR sI sR kS : term).
 
 Definition nslN := nroot.@"nsl".
 
@@ -28,15 +28,10 @@ Record sess_info : Type := SessInfo {
   si_resp_share : term;
 }.
 
-Definition si_key kI kR si :=
-  Spec.derive_key (Spec.of_list [TKey Seal kI; TKey Seal kR;
+Definition si_key skI skR si :=
+  Spec.derive_key (Spec.of_list [TKey Seal skI; TKey Seal skR;
                                  si_init_share si;
                                  si_resp_share si]).
-
-Definition nsl_session kI kR si : iProp :=
-  □ (public (TKey Open kI) → ▷ False) ∗
-  □ (public (TKey Open kR) → ▷ False) ∗
-  □ (public (si_key kI kR si) → ▷^2 False).
 
 Lemma nsl_session_agree kI1 kI2 kR1 kR2 si1 si2 :
   si_key kI1 kR1 si1 = si_key kI2 kR2 si2 →
@@ -47,41 +42,14 @@ case/Spec.of_list_inj.
 by case: si1 si2 => [??] [??] /= <- <- <- <-.
 Qed.
 
-Lemma nsl_session_public_key kI kR si :
-  nsl_session kI kR si -∗
-  public (si_key kI kR si) -∗
-  ▷^2 False.
-Proof. iIntros "(_ & _ & #H) #p_t". by iApply "H". Qed.
+Definition nonce_secrecy skA pkB : iProp :=
+  ∃ skB, ⌜pkB = TKey Seal skB⌝ ∗
+         (compromised_key skA ∨ compromised_key skB).
 
-Definition compromise pk : iProp :=
-  ∃ sk, ⌜pk = TKey Seal sk⌝ ∧ public (TKey Open sk).
-
-Lemma compromise_TKey sk :
-  compromise (TKey Seal sk) ⊣⊢ public (TKey Open sk).
-Proof.
-iSplit.
-- by iIntros "(%sk' & %e & #?)"; case: e => <-.
-- by iIntros "#p_dk"; iExists _; eauto.
-Qed.
-
-Lemma nsl_session_alloc kI kR si :
-  □ (public (TKey Open kI) → ▷ False) -∗
-  □ (public (TKey Open kR) → ▷ False) -∗
-  □ (public (si_init_share si) ↔
-       ▷ □ (public (TKey Open kI) ∨ public (TKey Open kR))) -∗
-  □ (public (si_resp_share si) ↔
-       ▷ □ (public (TKey Open kI) ∨ public (TKey Open kR))) ==∗
-  nsl_session kI kR si.
-Proof.
-iIntros "#s_dkI #s_dkR #s_nI #s_nR".
-iAssert (□ (public (si_key kI kR si) → ▷^2 False))%I as "#s_sk".
-{ iIntros "!> #p_sk".
-  rewrite public_derive_key public_of_list /=.
-  iDestruct "p_sk" as "(_ & _ & p_nI & _)".
-  by iDestruct ("s_nI" with "p_nI") as "[contra|contra]"; iNext;
-  [iApply "s_dkI"|iApply "s_dkR"]. }
-iModIntro. by do !iSplit => //.
-Qed.
+Lemma nonce_secrecyE skA skB :
+  nonce_secrecy skA (TKey Seal skB) ⊣⊢
+  compromised_key skA ∨ compromised_key skB.
+Proof. Admitted.
 
 (*
 
@@ -118,22 +86,21 @@ Definition resp : val := λ: "c" "skR",
   let: "sess_key" := derive_key (term_of_list ["pkI"; "pkR"; "nI"; "nR"]) in
   SOME ("pkI", "sess_key").
 
-Definition msg1_pred kR m1 : iProp := ∃ nI kI,
-  ⌜m1 = Spec.of_list [nI; TKey Seal kI]⌝ ∧
-  public (TKey Seal kI) ∧
-  (public nI ↔ ▷ □ (public (TKey Open kI) ∨ public (TKey Open kR))).
+Definition msg1_pred skR m1 : iProp := ∃ nI skI,
+  ⌜m1 = Spec.of_list [nI; TKey Seal skI]⌝ ∧
+  public (TKey Seal skI) ∧
+  (public nI ↔ ▷ □ nonce_secrecy skI (TKey Seal skR)).
 
-Definition msg2_pred kI m2 : iProp := ∃ nI nR kR,
+Definition msg2_pred skI m2 : iProp := ∃ nI nR skR,
   let sess_key :=
-    Spec.derive_key (Spec.of_list [TKey Seal kI; TKey Seal kR; nI; nR]) in
-  ⌜m2 = Spec.of_list [nI; nR; TKey Seal kR]⌝ ∧
-  (public (TKey Open kR) → ▷ False) ∧
-  (public nR ↔ ▷ □ (public (TKey Open kI) ∨ public (TKey Open kR))) ∧
-  term_meta nR (nroot.@"data") sess_key.
+    Spec.derive_key (Spec.of_list [TKey Seal skI; TKey Seal skR; nI; nR]) in
+  ⌜m2 = Spec.of_list [nI; nR; TKey Seal skR]⌝ ∧
+  (compromised_key skR → ▷ False) ∧
+  (public nR ↔ ▷ □ nonce_secrecy skR (TKey Seal skI)) ∧
+  term_meta nR (nroot.@"data") (TKey Seal skI).
 
-Definition msg3_pred kR nR : iProp := ∃ kI si,
-  term_meta nR (nroot.@"data") (si_key kI kR si) ∧
-  nsl_session kI kR si.
+Definition msg3_pred skR nR : iProp := ∃ skI,
+  term_meta nR (nroot.@"data") (TKey Seal skI).
 
 Definition nsl_ctx : iProp :=
   seal_pred (nslN.@"m1") msg1_pred ∧
@@ -160,53 +127,54 @@ Qed.
 Global Instance nsl_ctx_persistent : Persistent nsl_ctx.
 Proof. apply _. Qed.
 
-Lemma init_send_1 kI kR nI :
+Lemma init_send_1 skI skR nI :
   cryptis_ctx -∗
   nsl_ctx -∗
-  public (TKey Seal kI) -∗
-  □ (public (TKey Open kI) → ▷ False) -∗
-  public (TKey Seal kR) -∗
+  public (TKey Seal skI) -∗
+  □ (compromised_key skI → ▷ False) -∗
+  public (TKey Seal skR) -∗
   minted nI -∗
-  □ (public nI ↔ ▷ □ (public (TKey Open kI) ∨ public (TKey Open kR))) -∗
-  public (TSeal (TKey Seal kR) (Spec.tag (nslN.@"m1") (Spec.of_list [nI; TKey Seal kI]))).
+  □ (public nI ↔ ▷ □ nonce_secrecy skI (TKey Seal skR)) -∗
+  public (TSeal (TKey Seal skR) (Spec.tag (nslN.@"m1") (Spec.of_list [nI; TKey Seal skI]))).
 Proof.
 iIntros "#? (#? & _ & _) #p_ekI #s_dkI #p_ekR #m_nI #p_nI".
 iApply public_TSealIS; eauto.
 - iModIntro. by iExists _, _; iSplit; eauto.
 - by rewrite minted_of_list /=; eauto.
 - rewrite public_of_list /=. iIntros "!> #p_dkR".
-  do 2?iSplit => //. iApply "p_nI". by eauto.
+  do 2?iSplit => //. iApply "p_nI".
+  rewrite nonce_secrecyE /compromised_key. by eauto.
 Qed.
 
-Lemma resp_recv_1_send_2 pkI kR nI nR :
-  let sess_key := Spec.derive_key (Spec.of_list [pkI; TKey Seal kR; nI; nR]) in
-  public (TSeal (TKey Seal kR)
+Lemma resp_recv_1_send_2 pkI skR nI nR :
+  let sess_key := Spec.derive_key (Spec.of_list [pkI; TKey Seal skR; nI; nR]) in
+  public (TSeal (TKey Seal skR)
             (Spec.tag (nslN.@"m1")
                (Spec.of_list [nI; pkI]))) -∗
   term_token nR ⊤ -∗
   cryptis_ctx ∗
   nsl_ctx ∗
-  public (TKey Seal kR) ∗
-  □ (public (TKey Open kR) → ▷ False) ∗
+  public (TKey Seal skR) ∗
+  □ (compromised_key skR → ▷ False) ∗
   minted nR ∗
-  □ (public nR ↔ ▷ □ (compromise pkI ∨ public (TKey Open kR))) ={⊤}▷=∗
-  term_meta nR (nroot.@"data") sess_key ∗
+  □ (public nR ↔ ▷ □ nonce_secrecy skR pkI) ={⊤}▷=∗
+  term_meta nR (nroot.@"data") pkI ∗
   term_token nR (⊤ ∖ ↑nroot.@"data") ∗
   public pkI ∗
-  □ (▷ □ (compromise pkI ∨ public (TKey Open kR)) → public nI) ∗
+  □ (▷ □ nonce_secrecy skR pkI → public nI) ∗
   public (TSeal pkI
             (Spec.tag (nslN.@"m2")
-               (Spec.of_list [nI; nR; TKey Seal kR]))).
+               (Spec.of_list [nI; nR; TKey Seal skR]))).
 Proof.
 iIntros "%sess_key #p_m1 nR_token".
 iIntros "(#? & (#? & #? & _) & #p_ekR & #s_dkR & #m_nR & #p_nR)".
 rewrite (term_token_difference nR (↑nroot.@"data")) //.
 iDestruct "nR_token" as "[data nR_token]"; iFrame "nR_token".
-iMod (term_meta_set' (N := nroot.@"data") sess_key with "data")
+iMod (term_meta_set' (N := nroot.@"data") pkI with "data")
        as "[#meta _]"; first solve_ndisj.
 set m2 := Spec.of_list [_; _; _].
-iAssert (□ ∀ kI, ⌜pkI = TKey Seal kI⌝ → msg2_pred kI m2)%I as "#inv_m2".
-{ iIntros "!> %kI ->". rewrite /msg2_pred compromise_TKey. by eauto 13. }
+iAssert (□ ∀ skI, ⌜pkI = TKey Seal skI⌝ → msg2_pred skI m2)%I as "#inv_m2".
+{ iIntros "!> %skI ->". iExists nI, nR, skR. do !iSplit => //. }
 iDestruct (public_TSealE with "p_m1 [//]") as "[[_ fail]|succ]".
 - rewrite public_of_list /=. iDestruct "fail" as "(? & ? & _)".
   iIntros "!> !> !>". do !iSplit => //.
@@ -215,16 +183,17 @@ iDestruct (public_TSealE with "p_m1 [//]") as "[[_ fail]|succ]".
   + by iApply public_minted.
   + rewrite minted_of_list /=.
     by do !iSplit => //; iApply public_minted.
-  + iIntros "%kI %e". iSplit.
+  + iIntros "%skI %e". iSplit.
     * iModIntro. by iApply "inv_m2".
     * iIntros "!> #p_dkR". rewrite public_of_list /=.
-      do !iSplit => //. iApply "p_nR". rewrite {}e.
-      iLeft. iExists kI. by eauto.
+      do !iSplit => //. iApply "p_nR". iIntros "!> !>". rewrite {}e.
+      rewrite nonce_secrecyE. iRight. by iSplit.
 - iDestruct "succ" as "(#inv_m1 & m_m1 & _)". iIntros "!> !>".
-  iDestruct "inv_m1" as "(%nI' & %kI & %e & p_ekI & s_nI)".
+  iDestruct "inv_m1" as "(%nI' & %skI & %e & p_ekI & s_nI)".
   case/Spec.of_list_inj: e => <- -> {nI' pkI} in sess_key *.
   do 3!iSplitR => //.
-  { rewrite compromise_TKey. iIntros "!> !> #fail". by iApply "s_nI". }
+  { rewrite !nonce_secrecyE bi.or_comm.
+    iIntros "!> !> #fail". by iApply "s_nI". }
   iApply public_TSealIS => //.
   + by iApply public_minted.
   + iModIntro. by iApply "inv_m2".
@@ -232,29 +201,28 @@ iDestruct (public_TSealE with "p_m1 [//]") as "[[_ fail]|succ]".
     by do !iSplit => //; iApply public_minted.
   + iIntros "!> !> #p_dkR". rewrite public_of_list /=.
     do !iSplit => //.
-    * iApply "s_nI". by eauto.
-    * iApply "p_nR". iLeft. iExists kI. by eauto.
+    * iApply "s_nI". rewrite !nonce_secrecyE /compromised_key. by eauto.
+    * iApply "p_nR". rewrite !nonce_secrecyE /compromised_key. by eauto.
 Qed.
 
-Lemma init_recv_2_send_3 kI kR nI nR :
+Lemma init_recv_2_send_3 skI skR nI nR :
   let si := SessInfo nI nR in
-  public (TSeal (TKey Seal kI)
+  public (TSeal (TKey Seal skI)
             (Spec.tag (nslN.@"m2")
-               (Spec.of_list [nI; nR; TKey Seal kR]))) -∗
+               (Spec.of_list [nI; nR; TKey Seal skR]))) -∗
   term_token nI ⊤ -∗
   cryptis_ctx ∗
   nsl_ctx ∗
-  public (TKey Seal kI) ∗
-  public (TKey Seal kR) ∗
-  □ (public (TKey Open kI) → ▷ False) ∗
-  □ (public nI ↔ ▷ □ (public (TKey Open kI) ∨ public (TKey Open kR))) ={⊤}▷=∗
+  public (TKey Seal skI) ∗
+  public (TKey Seal skR) ∗
+  □ (compromised_key skI → ▷ False) ∗
+  □ (public nI ↔ ▷ □ nonce_secrecy skI (TKey Seal skR)) ={⊤}▷=∗
   minted nR ∗
-  public (TSeal (TKey Seal kR) (Spec.tag (nslN.@"m3") nR)) ∗
+  public (TSeal (TKey Seal skR) (Spec.tag (nslN.@"m3") nR)) ∗
   term_token nI (⊤ ∖ ↑nroot.@"data") ∗
-  (public (TKey Open kR) ∗ public (si_key kI kR si)
-   ∨ nsl_session kI kR si).
+  □ (public (si_key skI skR si) ↔ ▷ □ nonce_secrecy skI (TKey Seal skR)).
 Proof.
-iIntros "%si #p_m2 nI_token".
+iIntros "%si #p_m2 nI_token". rewrite nonce_secrecyE.
 iIntros "(#? & (_ & #? & #?) & #p_ekI & #p_ekR & #s_dkI & #s_nI)".
 rewrite (term_token_difference _ (↑nroot.@"data")) //.
 iDestruct "nI_token" as "[_ nI_token]". iFrame "nI_token".
@@ -262,87 +230,91 @@ iDestruct (public_TSealE with "p_m2 [//]") as "[fail|succ]".
 - rewrite !public_of_list /=.
   iDestruct "fail" as "(_ & p_nI & p_nR & _ & _)".
   iSpecialize ("s_nI" with "p_nI").
-  iIntros "!> !>". iDestruct "s_nI" as "#[contra|fail]".
-  { iDestruct ("s_dkI" with "contra") as ">[]". }
-  iIntros "!>". iSplit; first by iApply public_minted.
+  iIntros "!> !> !>". iSplit; first by iApply public_minted.
   iSplit.
   + iApply public_TSealIP => //. by rewrite public_tag.
-  + iLeft. do !iSplit => //.
-    rewrite public_derive_key public_of_list /=. by eauto.
+  + rewrite public_derive_key public_of_list /=.
+    iModIntro. iSplit; by eauto 10.
 - iDestruct "succ" as "(#inv_m2 & m_m2 & _)".
   rewrite minted_of_list /=. iDestruct "m_m2" as "(_ & m_nR & _)".
   iIntros "!> !>".
   iDestruct "inv_m2"
-    as "(%nI' & %nR' & %kR' & %e & s_dkR & s_nR & meta)".
-  case/Spec.of_list_inj: e => {nI' nR' kR'} <- <- <-.
-  iMod (nsl_session_alloc kI kR si with "[//] [//] [//] [//]")
-    as "#key_nR'" => //.
-  iFrame. iIntros "!>". iSplit => //.
-  iSplit.
+    as "(%nI' & %nR' & %skR' & %e & s_dkR & s_nR & meta)".
+  case/Spec.of_list_inj: e => {nI' nR' skR'} _ <- <-.
+  iModIntro. iSplit => //. iSplit.
   { iApply public_TSealIS => //.
     + by iApply public_minted.
-    + iIntros "!>". iExists kI, si. by eauto.
-    + iIntros "!> #p_dkR". iApply "s_nR". by eauto. }
-  iRight. by iFrame.
+    + iIntros "!>". by iExists skI.
+    + iIntros "!> #p_dkR". iApply "s_nR".
+      rewrite nonce_secrecyE /compromised_key. by eauto. }
+  rewrite public_derive_key public_of_list /=.
+  iModIntro. iSplit.
+  + iIntros "(_ & _ & #p_nI & _)". by iApply "s_nI".
+  + rewrite nonce_secrecyE bi.or_comm.
+    iIntros "#?". do !iSplit => //.
+    * by iApply "s_nI".
+    * by iApply "s_nR".
 Qed.
 
-Lemma resp_recv_3 pkI kR nI nR :
+Lemma resp_recv_3 pkI skR nI nR :
   let sess_key :=
-    Spec.derive_key (Spec.of_list [pkI; TKey Seal kR; nI; nR]) in
-  public (TSeal (TKey Seal kR) (Spec.tag (nslN.@"m3") nR)) -∗
+    Spec.derive_key (Spec.of_list [pkI; TKey Seal skR; nI; nR]) in
+  public (TSeal (TKey Seal skR) (Spec.tag (nslN.@"m3") nR)) -∗
   cryptis_ctx ∗
   nsl_ctx ∗
-  term_meta nR (nroot.@"data") sess_key ∗
+  term_meta nR (nroot.@"data") pkI ∗
   public pkI ∗
-  public (TKey Seal kR) ∗
-  □ (public (TKey Open kR) → ▷ False) ∗
-  □ (▷ □ (compromise pkI ∨ public (TKey Open kR)) → public nI) ∗
-  □ (public nR ↔ ▷ □ (compromise pkI ∨ public (TKey Open kR))) ={⊤}▷=∗ ∃ kI,
-  ⌜pkI = TKey Seal kI⌝ ∗
-  (public (TKey Open kI) ∗ public sess_key
-   ∨ nsl_session kI kR (SessInfo nI nR)).
+  public (TKey Seal skR) ∗
+  □ (compromised_key skR → ▷ False) ∗
+  □ (▷ □ nonce_secrecy skR pkI → public nI) ∗
+  □ (public nR ↔ ▷ □ nonce_secrecy skR pkI) ={⊤}▷=∗ ∃ skI,
+  ⌜pkI = TKey Seal skI⌝ ∗
+  □ (public (si_key skI skR (SessInfo nI nR)) ↔
+     ▷ □ nonce_secrecy skR pkI).
 Proof.
 iIntros "%sess_key #p_m3".
-iIntros "(#? & (_ & _ & #?) & #meta & #p_pkI & #p_pkR & #s_dkR & #p_nI & #s_nR)".
+iIntros "(#? & (_ & _ & #?) & #meta & #p_pkI & #p_pkR & #s_dkR & #s_nI & #s_nR)".
 iDestruct (public_TSealE with "p_m3 [//]") as "{p_m3} [[_ p_nR]|p_m3]".
-- iSpecialize ("s_nR" with "p_nR"). iIntros "!> !>".
-  iDestruct "s_nR" as "[(%kI & -> & #p_dkI)|#p_dkR]".
-  + iExists kI. rewrite public_derive_key public_of_list /= compromise_TKey.
-    iModIntro. iSplit => //. iLeft. do !iSplit => //.
-    iApply "p_nI". by eauto.
-  + by iDestruct ("s_dkR" with "p_dkR") as ">[]".
-- iDestruct "p_m3" as "(#inv_m3 & _)". iIntros "!> !>".
-  iDestruct "inv_m3" as "(%kI & %si & meta' & session)".
-  case: si => nI' nR'.
-  iPoseProof (term_meta_agree with "meta meta'") as "%e".
-  case/Spec.tag_inj: e => _ e.
-  case/Spec.of_list_inj: e => /= -> <- <-.
-  iModIntro. iExists kI. iSplit; eauto.
+- iSpecialize ("s_nR" with "p_nR"). iIntros "!> !> !>".
+  iDestruct "s_nR" as "(%skI & -> & fail)". iExists skI.
+  iSplit => //. rewrite nonce_secrecyE public_derive_key public_of_list /=.
+  iModIntro. iSplit.
+  + by eauto.
+  + iIntros "#comp". do !iSplit => //. by iApply "s_nI".
+- iDestruct "p_m3" as "(#inv_m3 & _)". iIntros "!> !> !>".
+  iDestruct "inv_m3" as "(%skI & meta')".
+  iPoseProof (term_meta_agree with "meta meta'") as "->".
+  iExists skI. iSplit => //. iModIntro.
+  rewrite public_derive_key public_of_list /=. iSplit.
+  + iIntros "(_ & _ & _ & #p_nR & _)". by iApply "s_nR".
+  + iIntros "#comp". do !iSplit => //.
+    * by iApply "s_nI".
+    * by iApply "s_nR".
 Qed.
 
 Ltac protocol_failure :=
   by intros; wp_pures; iApply ("Hpost" $! None); iFrame.
 
-Lemma wp_init c kI kR :
+Lemma wp_init c skI skR :
   channel c -∗
   cryptis_ctx -∗
   nsl_ctx -∗
-  public (TKey Seal kI) -∗
-  □ (public (TKey Open kI) → ▷ False) -∗
-  public (TKey Seal kR) -∗
+  public (TKey Seal skI) -∗
+  □ (compromised_key skI → ▷ False) -∗
+  public (TKey Seal skR) -∗
   {{{ True }}}
-    init c kI (TKey Seal kR)
-  {{{ si, RET (repr (si_key kI kR <$> si));
+    init c skI (TKey Seal skR)
+  {{{ si, RET (repr (si_key skI skR <$> si));
       if si is Some si then
-        let sk := si_key kI kR si in
+        let sk := si_key skI skR si in
         minted sk ∗
         term_token (si_init_share si) (⊤ ∖ ↑nroot.@"data") ∗
-        (public (TKey Open kR) ∗ public sk ∨ nsl_session kI kR si)
+        □ (public sk ↔ ▷ (compromised_key skI ∨ compromised_key skR))
       else True }}}.
 Proof.
-iIntros "#chan_c #ctx #ctx' #p_kI #s_kI #p_kR %Ψ !> _ Hpost".
+iIntros "#chan_c #ctx #ctx' #p_skI #s_skI #p_skR %Ψ !> _ Hpost".
 rewrite /init. wp_pures. wp_apply wp_pkey. wp_pures.
-wp_apply (wp_mknonce (λ _, public (TKey Open kI) ∨ public (TKey Open kR))%I
+wp_apply (wp_mknonce (λ _, nonce_secrecy skI (TKey Seal skR))%I
             (λ _, False)%I) => //.
 iIntros "%nI _ #m_nI #p_nI _ token".
 wp_pures. wp_list. wp_term_of_list. wp_apply wp_aenc => /=. wp_pures.
@@ -356,33 +328,35 @@ wp_eq_term e; last protocol_failure; subst nI'.
 wp_eq_term e; last protocol_failure; subst pkR'.
 iDestruct (init_recv_2_send_3 with "p_m2 [$] []") as ">H"; first by eauto 10.
 wp_pure.
-iMod "H" as "(#m_nR & #p_m3 & token & inv)".
+iMod "H" as "(#m_nR & #p_m3 & token & #inv)".
 wp_apply wp_aenc. wp_pures. wp_bind (send _ _). iApply wp_send => //.
 wp_list. wp_term_of_list. wp_apply wp_derive_key.
-set sess_key := Spec.derive_key (Spec.of_list [TKey Seal kI; _; _; _]).
+set sess_key := Spec.derive_key (Spec.of_list [TKey Seal skI; _; _; _]).
 wp_pures.
 iApply ("Hpost" $! (Some (SessInfo nI nR))). iModIntro. iFrame.
 rewrite minted_tag minted_of_list /=.
+iSplit; last first.
+{ by rewrite nonce_secrecyE bi.intuitionistic_intuitionistically. }
 by do !iSplit => //; iApply public_minted.
 Qed.
 
-Lemma wp_resp c kR :
+Lemma wp_resp c skR :
   channel c -∗
   cryptis_ctx -∗
   nsl_ctx -∗
-  public (TKey Seal kR) -∗
-  □ (public (TKey Open kR) → ▷ False) -∗
+  public (TKey Seal skR) -∗
+  □ (compromised_key skR → ▷ False) -∗
   {{{ True }}}
-    resp c kR
+    resp c skR
   {{{ ts, RET (repr ts);
-      if ts is Some (pkI, sk) then ∃ kI si,
-        ⌜pkI = TKey Seal kI⌝ ∗
-        ⌜sk = si_key kI kR si⌝ ∗
+      if ts is Some (pkI, sk) then ∃ skI si,
+        ⌜pkI = TKey Seal skI⌝ ∗
+        ⌜sk = si_key skI skR si⌝ ∗
         term_token (si_resp_share si) (⊤ ∖ ↑nroot.@"data") ∗
-        (public (TKey Open kI) ∗ public sk ∨ nsl_session kI kR si)
+        □ (public sk ↔ ▷ (compromised_key skI ∨ compromised_key skR))
       else True }}}.
 Proof.
-iIntros "#chan_c #ctx #ctx' #p_kR #honR %Ψ !> _ Hpost".
+iIntros "#chan_c #ctx #ctx' #p_skR #honR %Ψ !> _ Hpost".
 rewrite /resp. wp_pures. wp_apply wp_pkey. wp_pures.
 wp_bind (recv _); iApply wp_recv => //; iIntros (m1) "#p_m1".
 wp_adec m1; last protocol_failure.
@@ -394,9 +368,9 @@ iDestruct "m_m1" as "(_ & m_nI & m_pkI & _)".
 wp_pures. wp_bind (mknonce _).
 iApply (wp_mknonce_freshN
           ∅
-          (λ _, compromise pkI ∨ public (TKey Open kR))%I
+          (λ _, nonce_secrecy skR pkI)%I
           (λ _, False)%I
-          (λ nR, {[nR; Spec.derive_key (Spec.of_list [pkI; TKey Seal kR; nI; nR])]})) => //.
+          (λ nR, {[nR; Spec.derive_key (Spec.of_list [pkI; TKey Seal skR; nI; nR])]})) => //.
 - by iIntros "% %".
 - iIntros "%nR".
   rewrite big_sepS_union_pers !big_sepS_singleton minted_tag minted_of_list /=.
@@ -419,10 +393,12 @@ wp_pures. wp_bind (recv _). iApply wp_recv => //.
 iIntros "%m3 #p_m3". wp_adec m3; last protocol_failure.
 wp_eq_term e; last protocol_failure; subst m3.
 iPoseProof (resp_recv_3 with "p_m3 []") as ">finished"; first eauto 10.
-wp_pures. iMod "finished" as "(%kI & -> & finished)".
+wp_pures. iMod "finished" as "(%skI & -> & #finished)".
 wp_list. wp_term_of_list. wp_apply wp_derive_key. wp_pures.
-iApply ("Hpost" $! (Some (TKey Seal kI, sess_key))).
-iModIntro. iExists kI, (SessInfo nI nR). by eauto.
+iApply ("Hpost" $! (Some (TKey Seal skI, sess_key))).
+iModIntro. iExists skI, (SessInfo nI nR). iFrame.
+do !iSplit => //.
+by rewrite nonce_secrecyE bi.or_comm bi.intuitionistic_intuitionistically.
 Qed.
 
 Definition do_init_loop : val := rec: "loop" "c" "set" "skI" "pkR" :=
@@ -438,40 +414,40 @@ Definition do_init_loop : val := rec: "loop" "c" "set" "skI" "pkR" :=
    else #());;
    #().
 
-Definition do_init : val := λ: "c" "kI" "pkR",
+Definition do_init : val := λ: "c" "skI" "pkR",
   let: "set" := new_lock_term_set #() in
-  do_init_loop "c" "set" "kI" "pkR".
+  do_init_loop "c" "set" "skI" "pkR".
 
 Definition si_share_of rl :=
   if rl is Init then si_init_share else si_resp_share.
 
-Definition nsl_game_inv rl sk : iProp := ∃ kI kR si,
-  ⌜sk = si_key kI kR si⌝ ∧
+Definition nsl_game_inv rl sk : iProp := ∃ skI skR si,
+  ⌜sk = si_key skI skR si⌝ ∧
   term_meta (si_share_of rl si) (nroot.@"fresh") ().
 
-Lemma nsl_game_inv_fresh kI kR rl si E :
+Lemma nsl_game_inv_fresh skI skR rl si E :
   ↑nroot.@"fresh" ⊆ E →
   term_token (si_share_of rl si) E -∗
-  fresh_term (nsl_game_inv rl) (si_key kI kR si).
+  fresh_term (nsl_game_inv rl) (si_key skI skR si).
 Proof.
 iIntros "%sub token". iSplit.
-- iIntros "(%kI' & %kR' & %si' & %e & #meta)".
+- iIntros "(%skI' & %skR' & %si' & %e & #meta)".
   case/nsl_session_agree: e => _ _ <-.
   by iApply (term_meta_token with "token meta").
 - iMod (term_meta_set (nroot.@"fresh") () with "token") as "#?" => //.
-  iIntros "!> !>". iExists kI, kR, si. by eauto.
+  iIntros "!> !>". iExists skI, skR, si. by eauto.
 Qed.
 
-Lemma wp_do_init_loop c vset kI kR :
+Lemma wp_do_init_loop c vset skI skR :
   channel c -∗
   cryptis_ctx -∗
   nsl_ctx -∗
-  public (TKey Seal kI) -∗
-  □ (public (TKey Open kI) → ▷ False) -∗
-  □ (public (TKey Open kR) → ▷ False) -∗
+  public (TKey Seal skI) -∗
+  □ (compromised_key skI → ▷ False) -∗
+  □ (compromised_key skR → ▷ False) -∗
   is_lock_term_set (nsl_game_inv Init) vset -∗
   {{{ True }}}
-    do_init_loop c vset kI (TKey Seal kR)
+    do_init_loop c vset skI (TKey Seal skR)
   {{{ RET #(); True }}}.
 Proof.
 iIntros "#chan #? #? #p_pkI #s_skI #s_skR #set".
@@ -481,38 +457,39 @@ wp_rec; wp_pures; wp_apply wp_fork.
 wp_pures. wp_apply wp_recv => //.
 iIntros (ekR') "#p_ekR'".
 wp_pures; wp_bind (is_key _); iApply wp_is_key. wp_pures.
-case: Spec.is_keyP => [kt kR' eekR|_]; wp_pures; last by iApply "Hpost".
+case: Spec.is_keyP => [kt skR' eekR|_]; wp_pures; last by iApply "Hpost".
 wp_pures.
 case: bool_decide_reflect => [ekt|_]; wp_pures ; last by iApply "Hpost".
 case: kt eekR ekt => // -> _.
 wp_pures. wp_apply wp_init => //. iIntros "%ts tsP".
 case: ts=> [sk|] => /=; wp_pures; last by iApply "Hpost".
 wp_eq_term e; wp_pures; last by iApply "Hpost".
-case: e => <- {kR'}.
-iDestruct "tsP" as "(_ & token & [[#p_skR _]|#sess])".
-  iDestruct ("s_skR" with "p_skR") as ">[]".
-iPoseProof (@nsl_game_inv_fresh kI kR Init with "token")
+case: e => <- {skR'}.
+iDestruct "tsP" as "(_ & token & #s_sk)".
+iPoseProof (@nsl_game_inv_fresh skI skR Init with "token")
   as "fresh" => //; try solve_ndisj.
 wp_apply (wp_add_fresh_lock_term_set with "[$]"). iIntros "_".
 wp_pures. wp_apply wp_recv => //. iIntros "%guess #p_guess".
 wp_pures. wp_apply wp_assert.
 wp_eq_term e.
   rewrite -e.
-  iPoseProof (nsl_session_public_key with "sess p_guess") as "contra".
-  wp_pures.
-  by iDestruct "contra" as ">[]".
+  iPoseProof ("s_sk" with "p_guess") as "contra".
+  wp_pure _.
+  by iDestruct "contra" as "[contra|contra]";
+  [iDestruct ("s_skI" with "contra") as ">[]"|
+   iDestruct ("s_skR" with "contra") as ">[]"].
 wp_pures. iModIntro. iSplit => //. iNext. wp_pures. by iApply "Hpost".
 Qed.
 
-Lemma wp_do_init c kI kR :
+Lemma wp_do_init c skI skR :
   channel c -∗
   cryptis_ctx -∗
   nsl_ctx -∗
-  public (TKey Seal kI) -∗
-  □ (public (TKey Open kI) → ▷ False) -∗
-  □ (public (TKey Open kR) → ▷ False) -∗
+  public (TKey Seal skI) -∗
+  □ (compromised_key skI → ▷ False) -∗
+  □ (compromised_key skR → ▷ False) -∗
   {{{ True }}}
-    do_init c kI (TKey Seal kR)
+    do_init c skI (TKey Seal skR)
   {{{ RET #(); True }}}.
 Proof.
 iIntros "#chan #? #? #p_pkI #s_skI #s_skR %Φ _ !> post".
@@ -538,52 +515,52 @@ Definition do_resp : val := λ: "c" "skR" "pkI",
   let: "set" := new_lock_term_set #() in
   do_resp_loop "c" "set" "skR" "pkI".
 
-Lemma wp_do_resp_loop c set kI kR :
+Lemma wp_do_resp_loop c set skI skR :
   channel c -∗
   cryptis_ctx -∗
   nsl_ctx -∗
-  public (TKey Seal kR) -∗
-  □ (public (TKey Open kR) → ▷ False) -∗
-  □ (public (TKey Open kI) → ▷ False) -∗
+  public (TKey Seal skR) -∗
+  □ (compromised_key skR → ▷ False) -∗
+  □ (compromised_key skI → ▷ False) -∗
   is_lock_term_set (nsl_game_inv Resp) set -∗
   {{{ True }}}
-    do_resp_loop c set kR (TKey Seal kI)
+    do_resp_loop c set skR (TKey Seal skI)
   {{{ RET #(); True }}}.
 Proof.
-iIntros "#chan #? #? #p_ekR #s_dkR #s_dkI #set".
+iIntros "#chan #? #? #p_ekR #s_skR #s_skI #set".
 iLöb as "IH". iIntros "!> %Φ _ Hpost".
 wp_rec; wp_pures; wp_apply wp_fork.
 { iApply "IH" => //. }
 wp_pures. wp_apply wp_resp => //.
 iIntros "%res res".
 case: res => [[ekI' sk]|]; wp_pures; last by iApply "Hpost".
-iDestruct "res" as "(%kI' & %si & -> & -> & token & res)".
-iPoseProof (@nsl_game_inv_fresh kI' kR Resp with "token")
+iDestruct "res" as "(%skI' & %si & -> & -> & token & #res)".
+iPoseProof (@nsl_game_inv_fresh skI' skR Resp with "token")
   as "fresh" => //; try solve_ndisj.
 wp_apply (wp_add_fresh_lock_term_set with "[$]"). iIntros "_".
 wp_eq_term e; wp_pures; last by iApply "Hpost".
-case: e => <- {kI'}.
-iDestruct "res" as "[[#p_dkI _]|sess]".
-  iDestruct ("s_dkI" with "p_dkI") as ">[]".
+case: e => <- {skI'}.
 wp_pures. wp_apply wp_recv => //. iIntros "%guess #p_guess".
 wp_pures. wp_apply wp_assert.
 wp_eq_term e.
   rewrite -e.
-  iPoseProof (nsl_session_public_key with "sess p_guess") as "contra".
-  wp_pures.
-  by iDestruct "contra" as ">[]".
+  iPoseProof ("res" with "p_guess") as "contra".
+  wp_pure _.
+  by iDestruct "contra" as "[contra|contra]";
+  [iDestruct ("s_skI" with "contra") as ">[]"|
+   iDestruct ("s_skR" with "contra") as ">[]"].
 wp_pures. iModIntro. iSplit => //. iNext. wp_pures. by iApply "Hpost".
 Qed.
 
-Lemma wp_do_resp c kI kR :
+Lemma wp_do_resp c skI skR :
   channel c -∗
   cryptis_ctx -∗
   nsl_ctx -∗
-  public (TKey Seal kR) -∗
-  □ (public (TKey Open kR) → ▷ False) -∗
-  □ (public (TKey Open kI) → ▷ False) -∗
+  public (TKey Seal skR) -∗
+  □ (compromised_key skR → ▷ False) -∗
+  □ (compromised_key skI → ▷ False) -∗
   {{{ True }}}
-    do_resp c kR (TKey Seal kI)
+    do_resp c skR (TKey Seal skI)
   {{{ RET #(); True }}}.
 Proof.
 iIntros "#? #? #? #? #? #? %Φ _ !> post".
@@ -595,56 +572,40 @@ Qed.
 
 Definition game : val := λ: <>,
   let: "c"  := init_network #() in
-  let: "kI" := mkakey #() in
-  let: "kR" := mkakey #() in
-  let: "pkI" := pkey "kI" in
-  let: "pkR" := pkey "kR" in
+  let: "skI" := mkakey #() in
+  let: "skR" := mkakey #() in
+  let: "pkI" := pkey "skI" in
+  let: "pkR" := pkey "skR" in
   send "c" "pkI";;
   send "c" "pkR";;
-  Fork (do_init "c" "kI" "pkR");;
-  Fork (do_resp "c" "kR" "pkI").
+  Fork (do_init "c" "skI" "pkR");;
+  Fork (do_resp "c" "skR" "pkI").
 
 Lemma wp_game :
   cryptis_ctx -∗
   seal_pred_token ⊤ -∗
   key_pred_token (⊤ ∖ ↑nroot.@"keys") -∗
-  honest 0 ∅ -∗
-  ●Ph 0 -∗
   WP game #() {{ _, True }}.
 Proof.
-iIntros "#ctx enc_tok key_tok hon phase"; rewrite /game; wp_pures.
+iIntros "#ctx enc_tok key_tok"; rewrite /game; wp_pures.
 wp_apply wp_init_network => //. iIntros "%c #cP".
-wp_pures; wp_bind (mkakey _).
-iApply (wp_mkakey_phase with "[] [hon] phase"); eauto.
-iIntros "%kI #p_ekI hon phase tokenI". wp_pures.
-wp_bind (mkakey _). iApply (wp_mkakey_phase with "[] [hon] phase"); eauto.
-iIntros "%kR #p_ekR hon phase tokenR". wp_pures.
-wp_apply wp_pkey. wp_pures. set pkI := TKey Seal kI.
-set skI := TKey Open kI.
-wp_apply wp_pkey. wp_pures. set pkR := TKey Seal kR.
-set skR := TKey Open kR.
-iMod (freeze_honest with "[] hon phase") as "(hon & phase & sec)" => //; eauto.
+wp_pures. wp_apply (wp_mkakey with "[]"); eauto.
+iIntros "%skI #p_pkI #aencI secI tokenI".
+wp_pures. wp_apply (wp_mkakey with "[]"); eauto.
+iIntros "%skR #p_pkR #aencR secR tokenR".
+wp_pures. wp_apply wp_pkey. wp_pures. wp_apply wp_pkey. wp_pures.
+set pkI := TKey Seal skI.
+set pkR := TKey Seal skR.
+iMod (aenc_freeze_secret with "secI [//]") as "#?".
+iMod (aenc_freeze_secret with "secR [//]") as "#?".
 wp_pures; wp_bind (send _ _); iApply wp_send => //.
 wp_pures; wp_bind (send _ _); iApply wp_send => //.
-iMod "sec" as "sec".
-rewrite big_sepS_forall. wp_pures.
-iAssert (□ (public skI ↔ ▷ False))%I as "#s_dkI".
-  by iApply "sec"; iPureIntro; set_solver.
-iAssert (□ (public skR ↔ ▷ False))%I as "#s_dkR".
-  by iApply "sec"; iPureIntro; set_solver.
+wp_pures.
 iMod (nsl_alloc with "enc_tok") as "[#nsl_ctx _]" => //.
 wp_apply wp_fork.
-{ wp_apply wp_do_init => //.
-  { iIntros "!> #p_dkI".
-    iDestruct ("s_dkI" with "p_dkI") as ">[]". }
-  { iIntros "!> #p_dkR".
-    iDestruct ("s_dkR" with "p_dkR") as ">[]". } }
+{ wp_apply wp_do_init => //. }
 wp_pures. wp_apply wp_fork => //.
 wp_apply wp_do_resp => //.
-{ iIntros "!> #p_dkR".
-  iDestruct ("s_dkR" with "p_dkR") as ">[]". }
-{ iIntros "!> #p_dkI".
-  iDestruct ("s_dkI" with "p_dkI") as ">[]". }
 Qed.
 
 End NSL.
@@ -662,5 +623,5 @@ apply (adequate_not_stuck NotStuck _ _ (λ v _, True)) => //.
 apply: heap_adequacy.
 iIntros (?) "?".
 iMod (cryptisGS_alloc _) as (?) "(#ctx & enc_tok & key_tok & ? & hon & phase)".
-by iApply (wp_game with "ctx [enc_tok] [key_tok] [hon]").
+by iApply (wp_game with "ctx [enc_tok] [key_tok]").
 Qed.
